tests/test_scriptcert.py
@@ -2,31 +2,85 @@ from __future__ import annotations
 
 import unittest
 
-from src.scriptcert import Add, Mul, Neg, Num, Sub, check_semantic_preservation, compile_expr, eval_expr, parse_expr, run_program
+from src.scriptcert import (
+    Add,
+    MatchConst,
+    Mul,
+    Neg,
+    Num,
+    NumV,
+    OptChain,
+    PNum,
+    PUndef,
+    PWildcard,
+    SomeExpr,
+    SomeV,
+    Sub,
+    UNDEF,
+    check_semantic_preservation,
+    compile_expr,
+    eval_expr,
+    parse_expr,
+    run_program,
+)
 
 
 class ScriptCertTests(unittest.TestCase):
     def test_single_number(self) -> None:
         expr = Num(42)
-        self.assertEqual(eval_expr(expr), 42)
-        self.assertEqual(run_program(compile_expr(expr)), [42])
+        self.assertEqual(eval_expr(expr), NumV(42))
+        self.assertEqual(run_program(compile_expr(expr)), [NumV(42)])
         self.assertTrue(check_semantic_preservation(expr))
 
     def test_nested_addition(self) -> None:
         expr = Add(Num(2), Add(Num(3), Num(4)))
-        self.assertEqual(eval_expr(expr), 9)
-        self.assertEqual(run_program(compile_expr(expr)), [9])
+        self.assertEqual(eval_expr(expr), NumV(9))
+        self.assertEqual(run_program(compile_expr(expr)), [NumV(9)])
         self.assertTrue(check_semantic_preservation(expr))
 
     def test_sub_mul_neg(self) -> None:
         expr = Sub(Mul(Num(3), Num(5)), Neg(Num(2)))
-        self.assertEqual(eval_expr(expr), 17)
-        self.assertEqual(run_program(compile_expr(expr)), [17])
+        self.assertEqual(eval_expr(expr), NumV(17))
+        self.assertEqual(run_program(compile_expr(expr)), [NumV(17)])
         self.assertTrue(check_semantic_preservation(expr))
+
+    def test_optional_chaining(self) -> None:
+        expr = OptChain(SomeExpr(Add(Num(2), Num(5))))
+        self.assertEqual(eval_expr(expr), NumV(7))
+        self.assertTrue(check_semantic_preservation(expr))
+
+        miss_expr = OptChain(Num(9))
+        self.assertEqual(eval_expr(miss_expr), UNDEF)
+        self.assertTrue(check_semantic_preservation(miss_expr))
+
+    def test_pattern_matching(self) -> None:
+        expr = MatchConst(
+            OptChain(SomeExpr(Num(7))),
+            [(PNum(7), NumV(1)), (PUndef(), NumV(0)), (PWildcard(), NumV(-1))],
+            NumV(99),
+        )
+        self.assertEqual(eval_expr(expr), NumV(1))
+        self.assertTrue(check_semantic_preservation(expr))
+
+        undef_expr = MatchConst(OptChain(Num(3)), [(PNum(1), NumV(100))], NumV(-10))
+        self.assertEqual(eval_expr(undef_expr), NumV(-10))
+        self.assertTrue(check_semantic_preservation(undef_expr))
 
     def test_parser_for_new_ops(self) -> None:
         expr = parse_expr(["sub", ["mul", 6, ["neg", 2]], ["add", 1, 1]])
-        self.assertEqual(eval_expr(expr), -14)
+        self.assertEqual(eval_expr(expr), NumV(-14))
+        self.assertTrue(check_semantic_preservation(expr))
+
+    def test_parser_for_optional_chaining_and_match(self) -> None:
+        expr = parse_expr(
+            [
+                "match",
+                ["opt_chain", ["some", ["add", 3, 4]]],
+                [[["num", 7], 10], ["undef", 20], ["_", -1]],
+                0,
+            ]
+        )
+        self.assertEqual(eval_expr(expr), NumV(10))
         self.assertTrue(check_semantic_preservation(expr))
 
     def test_grid_of_small_values(self) -> None:
@@ -43,6 +97,16 @@ class ScriptCertTests(unittest.TestCase):
             for b in range(-2, 3):
                 expr = Sub(Mul(Num(a), Num(b)), Neg(Num(a)))
                 self.assertTrue(check_semantic_preservation(expr))
+
+    def test_grid_optional_chain_match(self) -> None:
+        for a in range(-2, 3):
+            expr = MatchConst(
+                OptChain(SomeExpr(Num(a))),
+                [(PNum(a), NumV(a + 1)), (PUndef(), NumV(0))],
+                NumV(-99),
+            )
+            self.assertEqual(eval_expr(expr), NumV(a + 1))
+            self.assertTrue(check_semantic_preservation(expr))
 
 
 if __name__ == "__main__":
