coq/JsPearl.v
@@ -2,45 +2,99 @@ From Coq Require Import ZArith List.
 Import ListNotations.
 Open Scope Z_scope.
 
+Inductive value : Type :=
+| VNum : Z -> value
+| VSome : value -> value
+| VUndef : value.
+
+Inductive pattern : Type :=
+| PMNum : Z -> pattern
+| PMSome : pattern
+| PMUndef : pattern
+| PMWild : pattern.
+
+Definition pattern_matches (p : pattern) (v : value) : bool :=
+  match p, v with
+  | PMNum n1, VNum n2 => Z.eqb n1 n2
+  | PMSome, VSome _ => true
+  | PMUndef, VUndef => true
+  | PMWild, _ => true
+  | _, _ => false
+  end.
+
+Fixpoint select_branch_value (v : value) (branches : list (pattern * value)) (dflt : value) : value :=
+  match branches with
+  | [] => dflt
+  | (p, rhs) :: tl => if pattern_matches p v then rhs else select_branch_value v tl dflt
+  end.
+
+Definition lift_binop (op : Z -> Z -> Z) (a b : value) : value :=
+  match a, b with
+  | VNum x, VNum y => VNum (op x y)
+  | _, _ => VUndef
+  end.
+
+Definition lift_unop (op : Z -> Z) (a : value) : value :=
+  match a with
+  | VNum x => VNum (op x)
+  | _ => VUndef
+  end.
+
+Definition opt_chain_value (a : value) : value :=
+  match a with
+  | VSome inner => inner
+  | _ => VUndef
+  end.
+
 (* Tiny JavaScript-like expression language. *)
 Inductive expr : Type :=
 | ENum : Z -> expr
 | EAdd : expr -> expr -> expr
 | ESub : expr -> expr -> expr
 | EMul : expr -> expr -> expr
-| ENeg : expr -> expr.
+| ENeg : expr -> expr
+| ESome : expr -> expr
+| EOptChain : expr -> expr
+| EMatchConst : expr -> list (pattern * value) -> value -> expr.
 
-Fixpoint eval (e : expr) : Z :=
+Fixpoint eval (e : expr) : value :=
   match e with
-  | ENum n => n
-  | EAdd a b => eval a + eval b
-  | ESub a b => eval a - eval b
-  | EMul a b => eval a * eval b
-  | ENeg a => - (eval a)
+  | ENum n => VNum n
+  | EAdd a b => lift_binop Z.add (eval a) (eval b)
+  | ESub a b => lift_binop Z.sub (eval a) (eval b)
+  | EMul a b => lift_binop Z.mul (eval a) (eval b)
+  | ENeg a => lift_unop Z.opp (eval a)
+  | ESome a => VSome (eval a)
+  | EOptChain a => opt_chain_value (eval a)
+  | EMatchConst scrutinee branches dflt =>
+      select_branch_value (eval scrutinee) branches dflt
   end.
 
 (* Tiny stack machine target language. *)
 Inductive instr : Type :=
-| IPush : Z -> instr
+| IPush : value -> instr
 | IAdd : instr
 | ISub : instr
 | IMul : instr
-| INeg : instr.
+| INeg : instr
+| IMakeSome : instr
+| IOptChain : instr
+| IMatchConst : list (pattern * value) -> value -> instr.
 
-Definition stack := list Z.
+Definition stack := list value.
 Definition program := list instr.
 
 Definition step (i : instr) (st : stack) : option stack :=
   match i, st with
-  | IPush n, _ => Some (n :: st)
-  | IAdd, x :: y :: st' => Some ((y + x) :: st')
-  | ISub, x :: y :: st' => Some ((y - x) :: st')
-  | IMul, x :: y :: st' => Some ((y * x) :: st')
-  | INeg, x :: st' => Some ((- x) :: st')
-  | IAdd, _ => None
-  | ISub, _ => None
-  | IMul, _ => None
-  | INeg, _ => None
+  | IPush v, _ => Some (v :: st)
+  | IAdd, x :: y :: st' => Some (lift_binop Z.add y x :: st')
+  | ISub, x :: y :: st' => Some (lift_binop Z.sub y x :: st')
+  | IMul, x :: y :: st' => Some (lift_binop Z.mul y x :: st')
+  | INeg, x :: st' => Some (lift_unop Z.opp x :: st')
+  | IMakeSome, x :: st' => Some (VSome x :: st')
+  | IOptChain, x :: st' => Some (opt_chain_value x :: st')
+  | IMatchConst branches dflt, x :: st' => Some (select_branch_value x branches dflt :: st')
+  | _, _ => None
   end.
 
 Fixpoint run (p : program) (st : stack) : option stack :=
@@ -55,11 +109,15 @@ Fixpoint run (p : program) (st : stack) : option stack :=
 
 Fixpoint compile (e : expr) : program :=
   match e with
-  | ENum n => [IPush n]
+  | ENum n => [IPush (VNum n)]
   | EAdd a b => compile a ++ compile b ++ [IAdd]
   | ESub a b => compile a ++ compile b ++ [ISub]
   | EMul a b => compile a ++ compile b ++ [IMul]
   | ENeg a => compile a ++ [INeg]
+  | ESome a => compile a ++ [IMakeSome]
+  | EOptChain a => compile a ++ [IOptChain]
+  | EMatchConst scrutinee branches dflt =>
+      compile scrutinee ++ [IMatchConst branches dflt]
   end.
 
 Lemma run_app : forall p q st st',
@@ -75,25 +133,35 @@ Qed.
 Theorem compile_correct_aux : forall e st,
   run (compile e) st = Some (eval e :: st).
 Proof.
-  induction e as [n|a IHa b IHb|a IHa b IHb|a IHa b IHb|a IHa]; intros st; simpl.
+  induction e as [n|a IHa b IHb|a IHa b IHb|a IHa b IHb|a IHa|a IHa|a IHa|scrutinee IHs branches dflt];
+    intros st; simpl.
   - reflexivity.
-  - rewrite run_app with (st' := [eval a]).
+  - rewrite run_app with (st' := eval a :: st).
     2: exact (IHa st).
-    rewrite run_app with (st' := [eval b; eval a]).
+    rewrite run_app with (st' := eval b :: eval a :: st).
     2: exact (IHb (eval a :: st)).
     simpl. reflexivity.
-  - rewrite run_app with (st' := [eval a]).
+  - rewrite run_app with (st' := eval a :: st).
     2: exact (IHa st).
-    rewrite run_app with (st' := [eval b; eval a]).
+    rewrite run_app with (st' := eval b :: eval a :: st).
     2: exact (IHb (eval a :: st)).
     simpl. reflexivity.
-  - rewrite run_app with (st' := [eval a]).
+  - rewrite run_app with (st' := eval a :: st).
     2: exact (IHa st).
-    rewrite run_app with (st' := [eval b; eval a]).
+    rewrite run_app with (st' := eval b :: eval a :: st).
     2: exact (IHb (eval a :: st)).
     simpl. reflexivity.
-  - rewrite run_app with (st' := [eval a]).
+  - rewrite run_app with (st' := eval a :: st).
     2: exact (IHa st).
+    simpl. reflexivity.
+  - rewrite run_app with (st' := eval a :: st).
+    2: exact (IHa st).
+    simpl. reflexivity.
+  - rewrite run_app with (st' := eval a :: st).
+    2: exact (IHa st).
+    simpl. reflexivity.
+  - rewrite run_app with (st' := eval scrutinee :: st).
+    2: exact (IHs st).
     simpl. reflexivity.
 Qed.
 
